theories/generic/utp_binding_fun.thy
@@ -2,13 +2,12 @@
 (* Title: utp/generic/utp_binding_fun.thy                                     *)
 (* Author: Frank Zeyda, University of York                                    *)
 (******************************************************************************)
+
+header {* Binding Functions *}
+
 theory utp_binding_fun
 imports utp_gen_pred
 begin
-
-section {* Binding Functions *}
-
-text {* TODO: Develop a tactic for membership to @{text "WF_BINDING_FUN"}. *}
 
 context GEN_PRED
 begin
@@ -21,38 +20,38 @@ theorem binding_fun_non_interfere1 :
 "\<lbrakk>x \<in> a\<rbrakk> \<Longrightarrow>
  (\<lambda> b . f (b x)) \<in> WF_BINDING_FUN a"
 apply (simp add: WF_BINDING_FUN_def)
-apply (simp add: binding_equiv_def)
+apply (simp add: beta_equiv_def)
 done
 
 theorem binding_fun_non_interfere2 :
 "\<lbrakk>x1 \<in> a; x2 \<in> a\<rbrakk> \<Longrightarrow>
  (\<lambda> b . f (b x1) (b x2)) \<in> WF_BINDING_FUN a"
 apply (simp add: WF_BINDING_FUN_def)
-apply (simp add: binding_equiv_def)
+apply (simp add: beta_equiv_def)
 done
 
 theorem binding_fun_non_interfere3 :
 "\<lbrakk>x1 \<in> a; x2 \<in> a; x3 \<in> a\<rbrakk> \<Longrightarrow>
  (\<lambda> b . f (b x1) (b x2) (b x3)) \<in> WF_BINDING_FUN a"
 apply (simp add: WF_BINDING_FUN_def)
-apply (simp add: binding_equiv_def)
+apply (simp add: beta_equiv_def)
 done
 
 theorem binding_fun_non_interfere4 :
 "\<lbrakk>x1 \<in> a; x2 \<in> a; x3 \<in> a; x4 \<in> a\<rbrakk> \<Longrightarrow>
  (\<lambda> b . f (b x1) (b x2) (b x3) (b x4)) \<in> WF_BINDING_FUN a"
 apply (simp add: WF_BINDING_FUN_def)
-apply (simp add: binding_equiv_def)
+apply (simp add: beta_equiv_def)
 done
 
 theorem binding_fun_non_interfere5 :
 "\<lbrakk>x1 \<in> a; x2 \<in> a; x3 \<in> a; x4 \<in> a; x5 \<in> a\<rbrakk> \<Longrightarrow>
  (\<lambda> b . f (b x1) (b x2) (b x3) (b x4) (b x5)) \<in> WF_BINDING_FUN a"
 apply (simp add: WF_BINDING_FUN_def)
-apply (simp add: binding_equiv_def)
+apply (simp add: beta_equiv_def)
 done
 
-(* Maybe the following are actually not needed in practice. *)
+-- {* The following may actually not be needed in practice. *}
 
 theorem binding_fun_and :
 "\<lbrakk>(\<lambda> b . f b) \<in> WF_BINDING_FUN a;
@@ -74,9 +73,11 @@ theorem binding_fun_not [simp] :
 apply (simp add: WF_BINDING_FUN_def)
 done
 
+text {* TODO: Develop a tactic for membership to @{text "WF_BINDING_FUN"}. *}
+
 subsection {* Proof Experiments *}
 
-theorem
+theorem LiftP_test_lemma :
 "v1 \<noteq> v2 \<longrightarrow> LiftP {x} (\<lambda> b . (b x) = v1 \<and> (b x) = v2) = false {x}"
 apply (subst LiftP_def)
 apply (simp_all)
