theories/generic/utp_eval_tactic.thy
@@ -2,11 +2,14 @@
 (* Title: utp/generic/utp_eval_tactic.thy                                     *)
 (* Author: Frank Zeyda, University of York                                    *)
 (******************************************************************************)
+
+header {* Proof Tactics *}
+
 theory utp_eval_tactic
 imports utp_gen_pred
 begin
 
-section {* Proof Tactic for Predicates *}
+text {* Interpretation-based proof tactic that facilitates logic proofs. *}
 
 context GEN_PRED
 begin
@@ -20,7 +23,7 @@ definition EvalP ::
  b \<in> WF_BINDING\<rbrakk> \<Longrightarrow>
  EvalP p b \<longleftrightarrow> b \<in> \<beta> p"
 
-subsection {* Fundamental Theorem *}
+subsection {* Introduction Theorems *}
 
 theorem EvalP_intro :
 "\<lbrakk>p1 \<in> WF_ALPHA_PREDICATE;
@@ -77,7 +80,7 @@ theorem EvalP_ExtP :
 "\<lbrakk>p \<in> WF_ALPHA_PREDICATE;
  a \<in> WF_ALPHABET;
  b \<in> WF_BINDING\<rbrakk> \<Longrightarrow>
- EvalP (p \<oplus> a) b = (EvalP p b)"
+ EvalP (p \<oplus>p a) b = (EvalP p b)"
 apply (simp add: EvalP_def)
 apply (simp add: ExtP_def)
 done
@@ -86,45 +89,51 @@ theorem EvalP_ResP :
 "\<lbrakk>p \<in> WF_ALPHA_PREDICATE;
  a \<in> WF_ALPHABET;
  b \<in> WF_BINDING\<rbrakk> \<Longrightarrow>
- EvalP (p \<ominus> a) b =
+ EvalP (p \<ominus>p a) b =
    (\<exists> b' \<in> WF_BINDING . b \<cong> b' on (\<alpha> p) - a \<and> EvalP p b')"
 apply (simp add: EvalP_def)
 apply (simp add: ResP_def)
 apply (safe)
 apply (rule_tac x = "b1" in bexI)
-apply (simp add: binding_equiv_comm)
-apply (simp add: WF_BINDING_member2)
+apply (simp add: beta_equiv_comm)
+apply (simp add: WF_BINDING_predicate)
 apply (rule_tac x = "b'" in bexI)
-apply (simp add: binding_equiv_comm)
+apply (simp add: beta_equiv_comm)
 apply (assumption)
 done
 
-(*
-  The theorem below is provable if we remove @{text "b \<in> WF_BINDING"} from the
-  assumptions in the definition of EvalP. However, it turns out that the law
-  is not as useful in practice because we have no general law that establishes
-  that the overridden binding is in @{text "WF_BINDING}. There is an open issue
-  how we recover the simplicity of the old approach using function override.
-*)
+text {* The next law relies on closure of @{term WF_BINDING} under override. *}
 
-(*
 theorem EvalP_ResP_override :
 "\<lbrakk>a \<in> WF_ALPHABET;
  p \<in> WF_ALPHA_PREDICATE;
  b \<in> WF_BINDING\<rbrakk> \<Longrightarrow>
- EvalP (p \<ominus> a) b =
-   (\<exists> b' \<in> WF_BINDING . EvalP p (b' \<oplus> b on (\<alpha> p) - a))"
+ EvalP (p \<ominus>p a) b = (\<exists> b' \<in> WF_BINDING . EvalP p (b \<oplus> b' on a))"
 apply (simp add: EvalP_def)
 apply (simp add: ResP_def)
 apply (safe)
+-- {* Subgoal 1 *}
 apply (rule_tac x = "b1" in bexI)
-apply (simp add: binding_equiv_override)
-apply (simp add: WF_BINDING_member2)
-apply (rule_tac x = "b' \<oplus> b on \<alpha> p - a" in bexI)
-apply (simp add: binding_equiv_def)
+apply (simp add: WF_ALPHA_PREDICATE_def WF_BINDING_SET_def)
+apply (clarify)
+apply (drule_tac x = "b1" in bspec)
 apply (assumption)
+apply (drule_tac x = "b \<oplus> b1 on a" in bspec)
+apply (auto) [1]
+apply (subgoal_tac "b1 \<cong> b \<oplus> b1 on a on \<alpha> p")
+apply (simp)
+apply (simp add: beta_equiv_def)
+apply (clarify)
+apply (case_tac "x \<in> a")
+apply (simp)
+apply (simp)
+apply (simp add: WF_BINDING_predicate)
+-- {* Subgoal 2 *}
+apply (rule_tac x = "b' \<oplus> b on - a" in bexI)
+apply (simp add: beta_equiv_def)
+apply (subst override_on_comm)
+apply (simp)
 done
-*)
 
 theorem EvalP_NotP :
 "\<lbrakk>p \<in> WF_ALPHA_PREDICATE;
@@ -181,6 +190,16 @@ apply (simp add: ExistsResP_def)
 apply (simp add: EvalP_ResP)
 done
 
+theorem EvalP_ExistsResP_override :
+"\<lbrakk>a \<in> WF_ALPHABET;
+ p \<in> WF_ALPHA_PREDICATE;
+ b \<in> WF_BINDING\<rbrakk> \<Longrightarrow>
+ EvalP (\<exists>-p a . p) b =
+   (\<exists> b' \<in> WF_BINDING . EvalP p (b \<oplus> b' on a))"
+apply (simp add: ExistsResP_def)
+apply (simp add: EvalP_ResP_override)
+done
+
 theorem EvalP_ForallResP :
 "\<lbrakk>a \<in> WF_ALPHABET;
  p \<in> WF_ALPHA_PREDICATE;
@@ -189,6 +208,16 @@ theorem EvalP_ForallResP :
    (\<forall> b' \<in> WF_BINDING . b \<cong> b' on (\<alpha> p) - a \<longrightarrow> EvalP p b')"
 apply (simp add: ForallResP_def)
 apply (simp add: EvalP_NotP EvalP_ExistsResP)
+done
+
+theorem EvalP_ForallResP_override :
+"\<lbrakk>a \<in> WF_ALPHABET;
+ p \<in> WF_ALPHA_PREDICATE;
+ b \<in> WF_BINDING\<rbrakk> \<Longrightarrow>
+ EvalP (\<forall>-p a . p) b =
+   (\<forall> b' \<in> WF_BINDING . EvalP p (b \<oplus> b' on a))"
+apply (simp add: ForallResP_def)
+apply (simp add: EvalP_NotP EvalP_ExistsResP_override)
 done
 
 theorem EvalP_ExistsP :
@@ -201,7 +230,17 @@ apply (simp add: ExistsP_def)
 apply (simp add: EvalP_ExtP EvalP_ExistsResP)
 done
 
-theorem EvalP_ForallP :
+theorem EvalP_ExistsP_override :
+"\<lbrakk>a \<in> WF_ALPHABET;
+ p \<in> WF_ALPHA_PREDICATE;
+ b \<in> WF_BINDING\<rbrakk> \<Longrightarrow>
+ EvalP (\<exists>p a . p) b =
+   (\<exists> b' \<in> WF_BINDING . EvalP p (b \<oplus> b' on a))"
+apply (simp add: ExistsP_def)
+apply (simp add: EvalP_ExtP EvalP_ExistsResP_override)
+done
+
+theorem EvalP_Forall :
 "\<lbrakk>a \<in> WF_ALPHABET;
  p \<in> WF_ALPHA_PREDICATE;
  b \<in> WF_BINDING\<rbrakk> \<Longrightarrow>
@@ -210,11 +249,21 @@ theorem EvalP_ForallP :
 apply (simp add: ForallP_def)
 apply (simp add: EvalP_ExtP EvalP_ForallResP)
 done
+
+theorem EvalP_ForallP_override :
+"\<lbrakk>a \<in> WF_ALPHABET;
+ p \<in> WF_ALPHA_PREDICATE;
+ b \<in> WF_BINDING\<rbrakk> \<Longrightarrow>
+ EvalP (\<forall>p a . p) b =
+   (\<forall> b' \<in> WF_BINDING . EvalP p (b \<oplus> b' on a))"
+apply (simp add: ForallP_def)
+apply (simp add: EvalP_ExtP EvalP_ForallResP_override)
+done
 end
 
 subsection {* Automatic Tactics *}
 
-subsubsection {* Theorem Attributes *}
+text {* Theorem Attributes *}
 
 ML {*
   structure eval =
@@ -235,16 +284,16 @@ declare EvalP_LiftP [eval]
 declare EvalP_TrueP [eval]
 declare EvalP_FalseP [eval]
 declare EvalP_ExtP [eval]
-declare EvalP_ResP [eval]
+declare EvalP_ResP_override [eval]
 declare EvalP_NotP [eval]
 declare EvalP_AndP [eval]
 declare EvalP_OrP [eval]
 declare EvalP_ImpliesP [eval]
 declare EvalP_IffP [eval]
-declare EvalP_ExistsResP [eval]
-declare EvalP_ForallResP [eval]
-declare EvalP_ExistsP [eval]
-declare EvalP_ForallP [eval]
+declare EvalP_ExistsResP_override [eval]
+declare EvalP_ForallResP_override [eval]
+declare EvalP_ExistsP_override [eval]
+declare EvalP_ForallP_override [eval]
 declare ClosureP_def [eval]
 declare RefP_def [eval]
 declare WF_ALPHABET_alphabet [eval]
@@ -254,19 +303,19 @@ declare Contingency_def [taut]
 declare Refinement_def [taut]
 end
 
-subsubsection {* Proof Methods *}
+text {* Proof Methods *}
 
 text {*
   We note that the proof methods are also generic and do not have to be
-  recreated for concrete instantiations of the @{text "GEN_PRED"} locale.
+  recreated for concrete instantiations of the @{term GEN_PRED} locale.
 *}
 
-ML{*
+ML {*
   fun utp_pred_eq_simpset ctxt =
     (simpset_of ctxt) addsimps (eval.get ctxt);
 *}
 
-ML{*
+ML {*
   fun utp_pred_taut_simpset ctxt =
     (utp_pred_eq_simpset ctxt) addsimps (taut.get ctxt);
 *}
@@ -277,7 +326,7 @@ method_setup utp_pred_eq_tac = {*
     SIMPLE_METHOD' (fn i =>
       CHANGED (asm_full_simp_tac
         (utp_pred_eq_simpset ctxt) i)))
-*} "Proof Tactic for Predicate Equalities"
+*} "proof tactic for predicate equalities"
 
 method_setup utp_pred_taut_tac = {*
   Attrib.thms >>
@@ -285,7 +334,7 @@ method_setup utp_pred_taut_tac = {*
     SIMPLE_METHOD' (fn i =>
       CHANGED (asm_full_simp_tac
         (utp_pred_taut_simpset ctxt) i)))
-*} "Proof Tactic for Predicate Tautologies"
+*} "proof tactic for predicate tautologies"
 
 text {* TODO: Integrate Holger's code for the simplifier to raise provisos. *}
 
