theories/generic/utp_function.thy
@@ -2,11 +2,12 @@
 (* Title: utp/generic/utp_function.thy                                        *)
 (* Author: Frank Zeyda, University of York                                    *)
 (******************************************************************************)
+
+header {* Predicate Functions *}
+
 theory utp_function
 imports utp_gen_pred
 begin
-
-section {* Functions on Predicates *}
 
 types ('VALUE, 'TYPE) ALPHA_FUNCTION =
   "('VALUE, 'TYPE) ALPHA_PREDICATE \<Rightarrow>
@@ -14,6 +15,7 @@ types ('VALUE, 'TYPE) ALPHA_FUNCTION =
 
 context GEN_PRED
 begin
+
 definition WF_ALPHA_FUNCTION :: "('VALUE, 'TYPE) ALPHA_FUNCTION set" where
 "WF_ALPHA_FUNCTION =
  {f . \<forall> p \<in> WF_ALPHA_PREDICATE . f p \<in> WF_ALPHA_PREDICATE}"
@@ -24,17 +26,14 @@ definition WF_ALPHA_FUNCTION_OVER ::
  WF_ALPHA_FUNCTION_OVER a =
  {f . \<forall> p \<in> WF_ALPHA_PREDICATE_OVER a . f p \<in> WF_ALPHA_PREDICATE}"
 
-text {* The following could be useful, this still needs to be explored! *}
-
 definition WF_ALPHA_FUNCTION_BETWEEN ::
   "['TYPE ALPHABET, 'TYPE ALPHABET] \<Rightarrow>
    ('VALUE, 'TYPE) ALPHA_FUNCTION set" where
-"\<lbrakk>a1 \<in> WF_ALPHABET;
- a2 \<in> WF_ALPHABET\<rbrakk> \<Longrightarrow>
+"\<lbrakk>a1 \<in> WF_ALPHABET; a2 \<in> WF_ALPHABET\<rbrakk> \<Longrightarrow>
  WF_ALPHA_FUNCTION_BETWEEN a1 a2 \<equiv>
  {f . \<forall> p \<in> WF_ALPHA_PREDICATE_OVER a1 . f p \<in> WF_ALPHA_PREDICATE_OVER a2}"
 
-section {* Restrictions *}
+subsection {* Restrictions *}
 
 definition IDEMPOTENT :: "('VALUE, 'TYPE) ALPHA_FUNCTION set" where
 "IDEMPOTENT = {f . \<forall> p \<in> WF_ALPHA_PREDICATE . f (f p) = f p}"
@@ -45,8 +44,7 @@ definition IDEMPOTENT_OVER ::
  IDEMPOTENT_OVER a = {f . \<forall> p \<in> WF_ALPHA_PREDICATE_OVER a . f (f p) = f p}"
 
 definition MONOTONIC :: "('VALUE, 'TYPE) ALPHA_FUNCTION set" where
-"MONOTONIC =
- {f \<in> WF_ALPHA_FUNCTION .
+"MONOTONIC = {f \<in> WF_ALPHA_FUNCTION .
    \<forall> a \<in> WF_ALPHABET .
    \<forall> p1 \<in> WF_ALPHA_PREDICATE_OVER a .
    \<forall> p2 \<in> WF_ALPHA_PREDICATE_OVER a . p1 \<sqsubseteq> p2 \<longrightarrow> f(p1) \<sqsubseteq> f(p2)}"
