theories/generic/utp_gen_laws.thy
@@ -1,0 +1,23 @@
+(******************************************************************************)
+(* Title: utp/generic/utp_gen_laws.thy                                        *)
+(* Author: Frank Zeyda, University of York                                    *)
+(******************************************************************************)
+
+header {* Generic Laws *}
+
+theory utp_gen_laws
+imports utp_eval_tactic
+begin
+
+context GEN_PRED
+begin
+theorem AndP_intro :
+"\<lbrakk>p1 \<in> WF_ALPHA_PREDICATE;
+ p2 \<in> WF_ALPHA_PREDICATE;
+ (\<alpha> p1) = (\<alpha> p2);
+ taut (p1 \<Rightarrow>p p2)\<rbrakk> \<Longrightarrow> p1 = (p1 \<and>p p2)"
+apply (utp_pred_taut_tac)
+apply (auto)
+done
+end
+end
