theories/generic/utp_generic.thy
@@ -2,18 +2,21 @@
 (* Title: utp/generic/utp_generic.thy                                         *)
 (* Author: Frank Zeyda, University of York                                    *)
 (******************************************************************************)
+
+header {* Meta-theory for Generics *}
+
 theory utp_generic
 imports
   utp_name
   utp_var
+  utp_value
+  utp_composite
   utp_alphabet
-  utp_abstract_value
-  utp_composite_value
   utp_gen_pred
-  utp_typed_pred
+  utp_gen_laws
   utp_eval_tactic
-  utp_function
   utp_binding_fun
+  utp_function
 begin
 
 text {* Meta-theory that imports all theories for generic models. *}
