theories/generic/utp_name.thy
@@ -2,18 +2,23 @@
 (* Title: utp/generic/utp_name.thy                                            *)
 (* Author: Frank Zeyda, University of York                                    *)
 (******************************************************************************)
+
+header {* Variable Names *}
+
 theory utp_name
 imports "../utp_common"
 begin
 
-section {* Variable Names *}
+subsection {* Subscripts *}
 
-subsection {* Encoding of Subscripts *}
+text {* Subscripts are encoded by virtue of a data type. *}
 
 datatype SUBSCRIPT =
   Sub "nat" | NoSub
 
-subsection {* Encoding of Names *}
+subsection {* Name Type *}
+
+text {* A record type is used to encode names. *}
 
 record NAME =
   name_str::"string"
@@ -21,6 +26,8 @@ record NAME =
   subscript::"SUBSCRIPT"
 
 subsection {* Restrictions *}
+
+text {* We only consider substitutions that are permutations. *}
 
 definition NAME_SUBST :: "(NAME \<Rightarrow> NAME) set" where
 "NAME_SUBST = bij"
