theories/theories/utp_rel.thy
@@ -2,11 +2,12 @@
 (* Title: utp/theories/utp_rel.thy                                            *)
 (* Author: Frank Zeyda, University of York                                    *)
 (******************************************************************************)
-theory utp_rel
-imports "../generic/utp_gen_pred"
-begin
 
-section {* Theory of Relations *}
+header {* Relational Predicates *}
+
+theory utp_rel
+imports "../generic/utp_gen_pred" "../generic/utp_eval_tactic"
+begin
 
 context GEN_PRED
 begin
@@ -74,21 +75,153 @@ definition SemiR ::
  COMPOSABLE (\<alpha> r1) (\<alpha> r1) \<longrightarrow>
  r1 ; r2 = (\<exists>-p dash ` (out (\<alpha> r1)) . r1[SS1] \<and>p r2[SS2])"
 
-subsubsection {* Theorems *}
+subsection {* Theorems *}
 
-theorem SubstP_closure :
+text {* Variable Substitution *}
+
+theorem VAR_SUBST_inv_closure [simp] :
+"ss \<in> VAR_SUBST \<Longrightarrow> (inv ss) \<in> VAR_SUBST"
+apply (simp add: VAR_SUBST_def)
+apply (safe)
+apply (auto intro: bij_imp_bij_inv)
+apply (drule_tac x = "inv ss v" in spec)
+apply (erule subst)
+apply (simp add: surj_f_inv_f bij_def)
+done
+
+theorem VAR_SUBST_inv_inv [simp] :
+"ss \<in> VAR_SUBST \<Longrightarrow> inv (inv ss) = ss"
+apply (simp add: VAR_SUBST_def)
+apply (simp add: inv_inv_eq)
+done
+
+theorem VAR_SUBST_ss_inv [simp] :
+"ss \<in> VAR_SUBST \<Longrightarrow> ss (inv ss x) = x"
+apply (simp add: VAR_SUBST_def)
+apply (simp add: surj_f_inv_f bij_def)
+done
+
+theorem VAR_SUBST_inv_ss [simp] :
+"ss \<in> VAR_SUBST \<Longrightarrow> inv ss (ss x) = x"
+apply (simp add: VAR_SUBST_def)
+apply (simp add: inv_f_f bij_def)
+done
+
+theorem VAR_SUBST_image_inv [simp] :
+"ss \<in> VAR_SUBST \<Longrightarrow> ss ` (inv ss) ` a = a"
+apply (simp add: image_def)
+apply (auto)
+done
+
+theorem VAR_SUBST_inv_image [simp] :
+"ss \<in> VAR_SUBST \<Longrightarrow> (inv ss) ` ss ` a = a"
+apply (simp add: image_def)
+apply (auto)
+done
+
+text {* Binding Substitution *}
+
+theorem SubstB_closure [simp] :
+"\<lbrakk>ss \<in> VAR_SUBST;
+ b \<in> WF_BINDING\<rbrakk> \<Longrightarrow>
+ SubstB ss b \<in> WF_BINDING"
+apply (simp add: SubstB_def WF_BINDING_def)
+apply (simp add: VAR_SUBST_def)
+apply (safe)
+apply (drule_tac x = "inv ss v" in spec)
+apply (subgoal_tac "type (inv ss v) = type v")
+apply (simp)
+apply (drule_tac x = "inv ss v" in spec)
+apply (erule subst)
+apply (simp add: surj_f_inv_f bij_def)
+done
+
+theorem SubstB_cancel1 [simp] :
+"\<lbrakk>ss \<in> VAR_SUBST;
+ b \<in> WF_BINDING\<rbrakk> \<Longrightarrow>
+ SubstB (inv ss) (SubstB ss b) = b"
+apply (subgoal_tac "SubstB ss b \<in> WF_BINDING")
+apply (simp add: SubstB_def)
+apply (rule ext)
+apply (simp_all)
+done
+
+theorem SubstB_cancel2 [simp] :
+"\<lbrakk>ss \<in> VAR_SUBST;
+ b \<in> WF_BINDING\<rbrakk> \<Longrightarrow>
+ SubstB ss (SubstB (inv ss) b) = b"
+apply (subgoal_tac "SubstB (inv ss) b \<in> WF_BINDING")
+apply (simp add: SubstB_def)
+apply (rule ext)
+apply (simp_all)
+done
+
+text {* Predicate Substitution *}
+
+theorem SubstP_closure_lemma :
+"\<lbrakk>ss \<in> VAR_SUBST;
+ b1 \<in> WF_BINDING;
+ b2 \<in> WF_BINDING\<rbrakk> \<Longrightarrow>
+ SubstB ss b1 \<cong> b2 on ss ` a \<longrightarrow> b1 \<cong> SubstB (inv ss) b2 on a"
+apply (simp add: beta_equiv_def)
+apply (simp add: SubstB_def)
+done
+
+theorem SubstP_closure [simp] :
 "\<lbrakk>p \<in> WF_ALPHA_PREDICATE;
  ss \<in> VAR_SUBST\<rbrakk> \<Longrightarrow>
  p[ss] \<in> WF_ALPHA_PREDICATE"
 apply (simp add: SubstP_def)
 apply (simp add: WF_ALPHA_PREDICATE_def)
 apply (safe)
-apply (simp add: WF_ALPHABET_def)
+-- {* Subgoal 1 *}
+apply (auto simp: WF_ALPHABET_def)
+-- {* Subgoal 2 *}
 apply (simp add: WF_BINDING_SET_def)
 apply (safe)
--- {* To prove this we need consistency of typing w.r.t. WF_BINDING! *}
--- {* This shows that we do need typing to be fixed in the locale. *}
-oops
+-- {* Subgoal 2.1 *}
+apply (subgoal_tac "xa \<in> WF_BINDING")
+apply (simp)
+apply (auto) [1]
+-- {* Subgoal 2.2 *}
+apply (simp (no_asm_simp) add: image_def)
+apply (rule_tac x = "SubstB (inv ss) b2" in bexI)
+apply (simp)
+apply (drule_tac x = "b1" in bspec)
+apply (assumption)
+apply (drule_tac x = "SubstB (inv ss) b2" in bspec)
+apply (simp)
+apply (subgoal_tac "b1 \<cong> SubstB (inv ss) b2 on \<alpha> p")
+apply (simp)
+apply (subst SubstP_closure_lemma)
+apply (auto)
+done
+
+theorem SubstP_alphabet [simp] :
+"\<lbrakk>p \<in> WF_ALPHA_PREDICATE;
+ ss \<in> VAR_SUBST\<rbrakk> \<Longrightarrow>
+ \<alpha> p[ss] = ss ` (\<alpha> p)"
+apply (simp add: SubstP_def)
+done
+
+theorem EvalP_SubstP [eval] :
+"\<lbrakk>p \<in> WF_ALPHA_PREDICATE;
+ ss \<in> VAR_SUBST;
+ b \<in> WF_BINDING\<rbrakk> \<Longrightarrow>
+ EvalP p[ss] b = EvalP p (SubstB (inv ss) b)"
+apply (simp add: EvalP_def)
+apply (simp add: SubstP_def)
+apply (simp add: image_def)
+apply (safe)
+apply (subgoal_tac "x \<in> WF_BINDING")
+apply (simp)
+apply (simp add: WF_BINDING_predicate)
+apply (rule_tac x = "SubstB (inv ss) b" in bexI)
+apply (simp)
+apply (assumption)
+done
+
+text {* Conditional *}
 
 theorem CondR_closure [simp] :
 "\<lbrakk>p1 \<in> WF_RELATION;
@@ -113,77 +246,33 @@ apply (simp add: WF_RELATION_def WF_CONDITION_def)
 apply (auto)
 done
 
+declare CondR_def [eval]
+
 subsection {* Proof Experiments *}
 
-theorem inj_on_override_on :
-"inj_on f a \<and> inj_on g b \<and> (f ` a) \<inter> (g ` b) = {} \<Longrightarrow>
- inj_on (f \<oplus> g on b) a"
-apply (simp add: inj_on_def)
-apply (safe)
-apply (case_tac "x \<in> b")
-apply (case_tac "y \<in> b")
-apply (simp_all)
-apply (rule_tac Q = "(f ` a) \<inter> (g ` b) = {}" in contrapos_pp)
-apply (assumption)
-apply (simp (no_asm_use) only: non_empty_exists)
-apply (rule_tac x = "g x" in exI)
-apply (safe)
-apply (simp)
-apply (thin_tac "g x = f y")
-apply (simp)
-apply (case_tac "y \<in> b")
-apply (simp_all)
-apply (rule_tac Q = "(f ` a) \<inter> (g ` b) = {}" in contrapos_pp)
-apply (assumption)
-apply (simp (no_asm_use) only: non_empty_exists)
-apply (rule_tac x = "f x" in exI)
-apply (safe)
-apply (thin_tac "f x = g y")
-apply (simp)
-apply (simp)
+theorem SubstP_lemma1 [simp] :
+"\<lbrakk>p \<in> WF_ALPHA_PREDICATE;
+ ss \<in> VAR_SUBST\<rbrakk> \<Longrightarrow>
+ p[ss][inv ss] = p"
+apply (utp_pred_taut_tac)
 done
 
-theorem inj_override_on :
-"inj_on f (-a) \<and> inj_on g a \<and> f ` (-a) \<inter> (g ` a) = {} \<Longrightarrow>
- inj f \<oplus> g on a"
-apply (simp add: inj_on_def)
-apply (safe)
-apply (case_tac "x \<in> a")
-apply (case_tac "y \<in> a")
-apply (simp_all)
-apply (rule_tac Q = "f ` (- a) \<inter> g ` a = {}" in contrapos_pp)
-apply (assumption)
-apply (simp (no_asm_use) only: non_empty_exists)
-apply (rule_tac x = "g x" in exI)
-apply (simp (no_asm_use))
-apply (safe)
-apply (simp)
-apply (thin_tac "g x = f y")
-apply (simp)
-apply (case_tac "y \<in> a")
-apply (simp_all)
-apply (rule_tac Q = "f ` (- a) \<inter> g ` a = {}" in contrapos_pp)
-apply (assumption)
-apply (simp (no_asm_use) only: non_empty_exists)
-apply (rule_tac x = "f x" in exI)
-apply (simp (no_asm_use))
-apply (safe)
-apply (thin_tac "f x = g y")
-apply (simp)
-apply (simp)
+theorem SubstP_lemma2 [simp] :
+"\<lbrakk>p1 \<in> WF_ALPHA_PREDICATE;
+ p2 \<in> WF_ALPHA_PREDICATE;
+ ss \<in> VAR_SUBST\<rbrakk> \<Longrightarrow>
+ (p1 \<and>p p2)[ss] = p1[ss] \<and>p p2[ss]"
+apply (utp_pred_eq_tac)
+apply (auto)
 done
 
-theorem bij_from_inj_on :
-"inj_on f a \<and> a \<inter> f ` a = {} \<longrightarrow>
- bij (id \<oplus> f on a) \<oplus> (inv f) on (f ` a)"
-apply (simp only: bij_def)
-apply (clarify)
-apply (rule conjI)
-apply (safe intro!: inj_override_on) [1]
-apply (safe intro!: inj_on_override_on) [1]
-apply (force)
-apply (force)
--- {* TODO: Finish the proof! *}
+theorem SubstP_lemma3 [simp] :
+"\<lbrakk>p \<in> WF_ALPHA_PREDICATE;
+ ss \<in> VAR_SUBST\<rbrakk> \<Longrightarrow>
+ taut [p] \<Leftrightarrow>p [p[ss]]"
+apply (utp_pred_taut_tac)
+apply (auto)
+-- {* This proof is more tricky! *}
 oops
 end
 end
