theories/utp.thy
@@ -2,6 +2,9 @@
 (* Title: utp/utp.thy                                                         *)
 (* Author: Frank Zeyda, University of York                                    *)
 (******************************************************************************)
+
+header {* Meta-theory for Everything *}
+
 theory utp
 imports
   "generic/utp_generic"
@@ -9,6 +12,6 @@ imports
   "theories/utp_theories"
 begin
 
-text {* Meta-theory that imports all UTP Isabelle theories. *}
+text {* Meta-theory that imports all theories of the UTP mechanisation. *}
 
 end
